@prefix : <http://www.oisrpg.com/rpg/ontology/> .
@prefix owl: <http://www.w3.org/2002/07/owl#> .
@prefix rdf: <http://www.w3.org/1999/02/22-rdf-syntax-ns#> .
@prefix xml: <http://www.w3.org/XML/1998/namespace> .
@prefix xsd: <http://www.w3.org/2001/XMLSchema#> .
@prefix rdfs: <http://www.w3.org/2000/01/rdf-schema#> .
@base <http://www.oisrpg.com/rpg/ontology/> .

<http://www.oisrpg.com/rpg/ontology/> rdf:type owl:Ontology .

#################################################################
#    Annotation properties
#################################################################

###  http://www.oisrpg.com/rpg/ontology/argument1
:argument1 rdf:type owl:AnnotationProperty .


###  http://www.oisrpg.com/rpg/ontology/argument2
:argument2 rdf:type owl:AnnotationProperty .


###  http://www.oisrpg.com/rpg/ontology/body
:body rdf:type owl:AnnotationProperty .


###  http://www.oisrpg.com/rpg/ontology/carringByPlayer
:carringByPlayer rdf:type owl:AnnotationProperty .


###  http://www.oisrpg.com/rpg/ontology/carryingByPlayer
:carryingByPlayer rdf:type owl:AnnotationProperty .


###  http://www.oisrpg.com/rpg/ontology/compostoPor
:compostoPor rdf:type owl:AnnotationProperty .


###  http://www.oisrpg.com/rpg/ontology/head
:head rdf:type owl:AnnotationProperty .


###  http://www.oisrpg.com/rpg/ontology/propertyPredicate
:propertyPredicate rdf:type owl:AnnotationProperty .


#################################################################
#    Data properties
#################################################################

###  http://www.oisrpg.com/rpg/ontology/AttributeDomain
:AttributeDomain rdf:type owl:DatatypeProperty ;
                 rdfs:domain :AttributeType ;
                 rdfs:range rdfs:Literal ;
                 rdfs:label "AttributeDomain"^^xsd:string .


###  http://www.oisrpg.com/rpg/ontology/#Physical
<http://www.oisrpg.com/rpg/ontology/#Physical> rdf:type owl:DatatypeProperty ;
                                               rdfs:subPropertyOf <http://www.oisrpg.com/rpg/ontology/#atributo> .


###  http://www.oisrpg.com/rpg/ontology/#atributo
<http://www.oisrpg.com/rpg/ontology/#atributo> rdf:type owl:DatatypeProperty ;
                                               rdfs:range xsd:integer .


###  http://www.oisrpg.com/rpg/ontology/#condicao
<http://www.oisrpg.com/rpg/ontology/#condicao> rdf:type owl:DatatypeProperty ;
                                               rdfs:subPropertyOf owl:topDataProperty ;
                                               rdfs:range xsd:string .


###  http://www.oisrpg.com/rpg/ontology/#dinheiro
<http://www.oisrpg.com/rpg/ontology/#dinheiro> rdf:type owl:DatatypeProperty ;
                                               rdfs:subPropertyOf owl:topDataProperty ;
                                               rdfs:range xsd:integer .


###  http://www.oisrpg.com/rpg/ontology/#experiência
<http://www.oisrpg.com/rpg/ontology/#experiência> rdf:type owl:DatatypeProperty ;
                                                  rdfs:subPropertyOf owl:topDataProperty ;
                                                  rdfs:range xsd:integer .


###  http://www.oisrpg.com/rpg/ontology/#mental
<http://www.oisrpg.com/rpg/ontology/#mental> rdf:type owl:DatatypeProperty ;
                                             rdfs:subPropertyOf <http://www.oisrpg.com/rpg/ontology/#atributo> .


###  http://www.oisrpg.com/rpg/ontology/#social
<http://www.oisrpg.com/rpg/ontology/#social> rdf:type owl:DatatypeProperty ;
                                             rdfs:subPropertyOf <http://www.oisrpg.com/rpg/ontology/#atributo> .


#################################################################
#    Classes
#################################################################

###  http://webprotege.stanford.edu/R15FH8CqRf3LGfLzttNvG9
<http://webprotege.stanford.edu/R15FH8CqRf3LGfLzttNvG9> rdf:type owl:Class ;
                                                        rdfs:subClassOf owl:Thing ;
                                                        rdfs:comment "Experience is used to upgrade and promote character enhancements"^^xsd:string ;
                                                        rdfs:label "Experience" .


###  http://webprotege.stanford.edu/R7AXrceSxSFcYRexGXJRk8x
<http://webprotege.stanford.edu/R7AXrceSxSFcYRexGXJRk8x> rdf:type owl:Class ;
                                                         rdfs:comment "Set of all elements linked about RPG"^^xsd:string ;
                                                         rdfs:label "Game" .


###  http://webprotege.stanford.edu/R7JTvOGeP4ORv7sbETcVXzS
<http://webprotege.stanford.edu/R7JTvOGeP4ORv7sbETcVXzS> rdf:type owl:Class ;
                                                         rdfs:subClassOf owl:Thing ;
                                                         rdfs:comment "Magazines have similar functions as books"^^xsd:string ;
                                                         rdfs:label "Magazine" .


###  http://webprotege.stanford.edu/R7P8ohrOIuRwoGanOBZy5i5
<http://webprotege.stanford.edu/R7P8ohrOIuRwoGanOBZy5i5> rdf:type owl:Class ;
                                                         rdfs:subClassOf owl:Thing ;
                                                         rdfs:comment "An adventure is a medium-sized story with middle beginning and end. An adventure can have a series of missions."^^xsd:string ;
                                                         rdfs:label "Adventure" .


###  http://webprotege.stanford.edu/R7XeyMKtcLS9AApz6EsW3Mx
<http://webprotege.stanford.edu/R7XeyMKtcLS9AApz6EsW3Mx> rdf:type owl:Class ;
                                                         rdfs:subClassOf owl:Thing ;
                                                         rdfs:comment "Representation of variables that define states or capacities of characters or of other elements within the rules in game"^^xsd:string ;
                                                         rdfs:label "Attribute" .


###  http://webprotege.stanford.edu/R83r9r1OlpKZHpNZcOhZNd
<http://webprotege.stanford.edu/R83r9r1OlpKZHpNZcOhZNd> rdf:type owl:Class ;
                                                        rdfs:subClassOf owl:Thing ;
                                                        rdfs:comment "Posts are informations about something. In PBF (Play-By-Forum), a post can represent description part of story."^^xsd:string ;
                                                        rdfs:label "Post" .


###  http://webprotege.stanford.edu/R8FbgJBSoBYuxDiHbyha7gG
<http://webprotege.stanford.edu/R8FbgJBSoBYuxDiHbyha7gG> rdf:type owl:Class ;
                                                         rdfs:subClassOf owl:Thing ;
                                                         rdfs:comment "Any character within a video game. The character could be playable or non playable (NPC)."^^xsd:string ;
                                                         rdfs:label "Character" ;
                                                         rdfs:seeAlso <http://autosemanticgame.institutedigitalgames.com/ontologies/game-character-ontology/> .


###  http://webprotege.stanford.edu/R8JJF2fxIyFyl1ONBXkWRFg
<http://webprotege.stanford.edu/R8JJF2fxIyFyl1ONBXkWRFg> rdf:type owl:Class ;
                                                         rdfs:comment "Combat maneuver to inflict damage"^^xsd:string ;
                                                         rdfs:label "Attack" .


###  http://webprotege.stanford.edu/R8LIplSgvLVMLURHdxjW9H1
<http://webprotege.stanford.edu/R8LIplSgvLVMLURHdxjW9H1> rdf:type owl:Class ;
                                                         rdfs:subClassOf owl:Thing ;
                                                         rdfs:comment "This category represents all entities in game, like: characters, places, objects, vehicles etc. This is a important abstract concept, because a entity can be act in the world in differents ways. For example: a horse can be seen like a vehicle, a character, object, or a place."^^xsd:string ;
                                                         rdfs:label "Entity" .


###  http://webprotege.stanford.edu/R8MiBfr3nJ6OUXJxsV5qH5D
<http://webprotege.stanford.edu/R8MiBfr3nJ6OUXJxsV5qH5D> rdf:type owl:Class ;
                                                         rdfs:comment "A sequence of actions for resolution of conflict, consisting of attacks and defense, but can has others maneuvers"^^xsd:string ;
                                                         rdfs:label "Combat" .


###  http://webprotege.stanford.edu/R8N0jZEDD7OVy9S6oLpXl88
<http://webprotege.stanford.edu/R8N0jZEDD7OVy9S6oLpXl88> rdf:type owl:Class ;
                                                         rdfs:subClassOf owl:Thing ;
                                                         rdfs:comment "Generator of random values, in tabletop RPG are commonly represented by polyhedral dice. Others ways for generate random numbers are possible like to use cards, coins and among others."^^xsd:string ;
                                                         rdfs:label "Dice" .


###  http://webprotege.stanford.edu/R8PptZazgxr1aCddeOhCDJN
<http://webprotege.stanford.edu/R8PptZazgxr1aCddeOhCDJN> rdf:type owl:Class ;
                                                         rdfs:subClassOf owl:Thing ;
                                                         rdfs:comment "Conflicts between players and NPCs are called encounters in which solving one or more problems is required. Such resolution may occur with or without combat."^^xsd:string ;
                                                         rdfs:label "Encounter" .


###  http://webprotege.stanford.edu/R8mpRbvmIOiJVQxBnxeSPzE
<http://webprotege.stanford.edu/R8mpRbvmIOiJVQxBnxeSPzE> rdf:type owl:Class ;
                                                         rdfs:subClassOf owl:Thing ;
                                                         rdfs:comment "Virtual environment for discussing or playing RPG matches (PBF, play-by-forum)"^^xsd:string ;
                                                         rdfs:label "Forum" .


###  http://webprotege.stanford.edu/R8owD02ngGvN11OLF5dhH6T
<http://webprotege.stanford.edu/R8owD02ngGvN11OLF5dhH6T> rdf:type owl:Class ;
                                                         rdfs:subClassOf owl:Thing ;
                                                         rdfs:comment "The Person class represents people. Something is a Person if it is a person. We don't nitpic about whether they're alive, dead, real, or imaginary. The Person class is a sub-class of the Agent class, since all people are considered 'agents' in FOAF."^^xsd:string ;
                                                         rdfs:label "Person" ;
                                                         rdfs:seeAlso <http://xmlns.com/foaf/spec/#term_Person> .


###  http://webprotege.stanford.edu/R8sQJeh6T4232sD80FRLEWb
<http://webprotege.stanford.edu/R8sQJeh6T4232sD80FRLEWb> rdf:type owl:Class ;
                                                         rdfs:subClassOf owl:Thing ;
                                                         rdfs:comment "News about realeses and updating from RPG"^^xsd:string ;
                                                         rdfs:label "News" .


###  http://webprotege.stanford.edu/R99rfdwFOjAPAIquXEPJS8Y
<http://webprotege.stanford.edu/R99rfdwFOjAPAIquXEPJS8Y> rdf:type owl:Class ;
                                                         rdfs:comment "Attributes wich specifies some states in game, including data about players"^^xsd:string ;
                                                         rdfs:label "AttributeDomain" .


###  http://webprotege.stanford.edu/R9PhYDVQV1tlQjuglIaL8qy
<http://webprotege.stanford.edu/R9PhYDVQV1tlQjuglIaL8qy> rdf:type owl:Class ;
                                                         rdfs:subClassOf owl:Thing ;
                                                         rdfs:comment "The scenario consists of all the entities that make up the universe of the game. The scenario includes: characters, ambiences, items, important events, that is, it has many of the narrative components of the game, while the system includes its rules."^^xsd:string ;
                                                         rdfs:label "Scenario" .


###  http://webprotege.stanford.edu/R9ZKeMKdDr8NdGk7uvtzrVC
<http://webprotege.stanford.edu/R9ZKeMKdDr8NdGk7uvtzrVC> rdf:type owl:Class ;
                                                         rdfs:subClassOf owl:Thing ;
                                                         rdfs:comment "Materials for studying rules, scenarios or to enable or discuss games"^^xsd:string ;
                                                         rdfs:label "Material" .


###  http://webprotege.stanford.edu/R9apHvU51re1QhRq2m16dMY
<http://webprotege.stanford.edu/R9apHvU51re1QhRq2m16dMY> rdf:type owl:Class ;
                                                         rdfs:subClassOf owl:Thing ;
                                                         rdfs:comment "Objects are items, equipments, or any element can be possed for someone."^^xsd:string ;
                                                         rdfs:label "Object" .


###  http://webprotege.stanford.edu/R9l3Pj6YpnzT4dR44bpjNOk
<http://webprotege.stanford.edu/R9l3Pj6YpnzT4dR44bpjNOk> rdf:type owl:Class ;
                                                         rdfs:comment "Others combat maneuvers which are not attack or defense, depending rules, like: dodge, flirt etc"^^xsd:string ;
                                                         rdfs:label "Other<Mode>" .


###  http://webprotege.stanford.edu/RB1IMjhjmZLzqrxsSab1HIc
<http://webprotege.stanford.edu/RB1IMjhjmZLzqrxsSab1HIc> rdf:type owl:Class ;
                                                         rdfs:comment "Planning is abstract class about with a set plan"^^xsd:string ;
                                                         rdfs:label "Planning" .


###  http://webprotege.stanford.edu/RBIWNvUrhhbbTMWb8AtWVei
<http://webprotege.stanford.edu/RBIWNvUrhhbbTMWb8AtWVei> rdf:type owl:Class ;
                                                         rdfs:subClassOf owl:Thing ;
                                                         rdfs:comment "Items are objects which can use in limited use, commonly is not used for damage. Like: potions, foods, poisons, etc."^^xsd:string ;
                                                         rdfs:label "Consumable" .


###  http://webprotege.stanford.edu/RBJDzlZERfgjfNeb2feN7PY
<http://webprotege.stanford.edu/RBJDzlZERfgjfNeb2feN7PY> rdf:type owl:Class ;
                                                         rdfs:subClassOf owl:Thing ;
                                                         rdfs:comment "Money for change items or others resources in game"^^xsd:string ;
                                                         rdfs:label "Money" .


###  http://webprotege.stanford.edu/RBVzgWkuTx69LsMzLQlIh3V
<http://webprotege.stanford.edu/RBVzgWkuTx69LsMzLQlIh3V> rdf:type owl:Class ;
                                                         rdfs:subClassOf owl:Thing ;
                                                         rdfs:comment "A plan is a set of actions considering its conditions and states to realize it"^^xsd:string ;
                                                         rdfs:label "Plan" .


###  http://webprotege.stanford.edu/RBepuHBNeISOA5C4aifpWhC
<http://webprotege.stanford.edu/RBepuHBNeISOA5C4aifpWhC> rdf:type owl:Class ;
                                                         rdfs:subClassOf owl:Thing ;
                                                         rdfs:comment "Condition is a set of constraints given a set of specific states."^^xsd:string ;
                                                         rdfs:label "Condition" .


###  http://webprotege.stanford.edu/RBwu10WmsskhzXBU3m7Zhhp
<http://webprotege.stanford.edu/RBwu10WmsskhzXBU3m7Zhhp> rdf:type owl:Class ;
                                                         rdfs:label "Resource" .


###  http://webprotege.stanford.edu/RCI6QrNhaDuqP9Lp63E9PKj
<http://webprotege.stanford.edu/RCI6QrNhaDuqP9Lp63E9PKj> rdf:type owl:Class ;
                                                         rdfs:subClassOf owl:Thing ;
                                                         rdfs:comment "Goals are defined by states to be achieved. Such goals can be defined within missions or discoveries in planning."^^xsd:string ;
                                                         rdfs:label "Goal" ;
                                                         rdfs:seeAlso <http://dev.nemo.inf.ufes.br/seon/UFO.html#UFO_Appointment+Goal_detail> .


###  http://webprotege.stanford.edu/RCTjweIOHzvqbViwGKHIIkD
<http://webprotege.stanford.edu/RCTjweIOHzvqbViwGKHIIkD> rdf:type owl:Class ;
                                                         rdfs:subClassOf owl:Thing ;
                                                         rdfs:comment "Human player in game. This entity controls PC (Player Character)."^^xsd:string ;
                                                         rdfs:label "Player" .


###  http://webprotege.stanford.edu/RCY5oKY95V0v1JkBMxZmtVp
<http://webprotege.stanford.edu/RCY5oKY95V0v1JkBMxZmtVp> rdf:type owl:Class ;
                                                         rdfs:comment "Test is a event that defines a success or fail in action. Tests commonly are random and are affected by attributes and states of the world."^^xsd:string ;
                                                         rdfs:label "Test" .


###  http://webprotege.stanford.edu/RCdJWxEniRbtosLi5ewWu8
<http://webprotege.stanford.edu/RCdJWxEniRbtosLi5ewWu8> rdf:type owl:Class ;
                                                        rdfs:subClassOf owl:Thing ;
                                                        rdfs:comment "A non-player character (NPC), also known as a non-playable character, is any character in a game which is not controlled by a player. In video games, this usually means a character controlled by the computer via algorithmic, predetermined or responsive behavior, but not necessarily true artificial intelligence. In traditional tabletop role-playing games, the term applies to characters controlled by the gamemaster or referee, rather than another player."^^xsd:string ;
                                                        rdfs:isDefinedBy <https://en.wikipedia.org/wiki/Non-player_character> ;
                                                        rdfs:label "NPC" ;
                                                        rdfs:seeAlso <http://dbpedia.org/page/Non-player_character> .


###  http://webprotege.stanford.edu/RCiUQ785q93mV1CxvSPsh1c
<http://webprotege.stanford.edu/RCiUQ785q93mV1CxvSPsh1c> rdf:type owl:Class ;
                                                         rdfs:comment "Equipment items are commonly wearable items which a character carry with itself. For example: weapons, armors, clothes, jewels, hats, etc."^^xsd:string ;
                                                         rdfs:label "Equipment" .


###  http://webprotege.stanford.edu/RCpvec4ghhf9hxQU95nkVCg
<http://webprotege.stanford.edu/RCpvec4ghhf9hxQU95nkVCg> rdf:type owl:Class ;
                                                         rdfs:subClassOf owl:Thing ;
                                                         rdfs:comment "Combat maneuver to defense against attacks"^^xsd:string ;
                                                         rdfs:label "Defense" .


###  http://webprotege.stanford.edu/RCqhga9AOxtzPBLBrat4d9c
<http://webprotege.stanford.edu/RCqhga9AOxtzPBLBrat4d9c> rdf:type owl:Class ;
                                                         rdfs:comment "System is set of rules from games"^^xsd:string ;
                                                         rdfs:label "System" .


###  http://webprotege.stanford.edu/RCw4khzIWoWmlUpbMNFRBO1
<http://webprotege.stanford.edu/RCw4khzIWoWmlUpbMNFRBO1> rdf:type owl:Class ;
                                                         rdfs:subClassOf owl:Thing ;
                                                         rdfs:comment "Session is an abstraction of time in game. For example, in digital games online, session starts in sign in and end in sign out. In Tabletop RPGs, session is when players init game match and end when they stop, but can be restarted the same adventure in another day."^^xsd:string ;
                                                         rdfs:label "Session" .


###  http://webprotege.stanford.edu/RDNuLunF6fRDQgcNlhTW6q3
<http://webprotege.stanford.edu/RDNuLunF6fRDQgcNlhTW6q3> rdf:type owl:Class ;
                                                         rdfs:comment "Events are individuals composed by temporal parts, they happen in time in the sense that they extend in time accumulating temporal parts. An example of an Event is a business process."^^xsd:string ;
                                                         rdfs:label "Event" ;
                                                         rdfs:seeAlso <https://ontology.com.br/ufo/ufo-b/spec/index.html> .


###  http://webprotege.stanford.edu/RDVDhmPb7EoC5MWHeIC7Rck
<http://webprotege.stanford.edu/RDVDhmPb7EoC5MWHeIC7Rck> rdf:type owl:Class ;
                                                         rdfs:comment "Sites are web pages"^^xsd:string ;
                                                         rdfs:label "Site" .


###  http://webprotege.stanford.edu/RGbugNys18CPGHzQAHG1hG
<http://webprotege.stanford.edu/RGbugNys18CPGHzQAHG1hG> rdf:type owl:Class ;
                                                        rdfs:subClassOf owl:Thing ;
                                                        rdfs:comment "Objects which are not defined like equipments or items. Etc can be collectable objects or objects needed for quests but which has not useful for other situations."^^xsd:string ;
                                                        rdfs:label "Etc" .


###  http://webprotege.stanford.edu/RYRe91IVY7mC7D7hkHS5Ai
<http://webprotege.stanford.edu/RYRe91IVY7mC7D7hkHS5Ai> rdf:type owl:Class ;
                                                        rdfs:subClassOf owl:Thing ;
                                                        rdfs:comment "A campaign is a long story or a set of adventures. In tabletop RPGs campaigns have big changes in scenario and in characters."^^xsd:string ;
                                                        rdfs:label "Campaign" .


###  http://webprotege.stanford.edu/RejpwDKlgIeVpHgAS5w6Ob
<http://webprotege.stanford.edu/RejpwDKlgIeVpHgAS5w6Ob> rdf:type owl:Class ;
                                                        rdfs:subClassOf owl:Thing ;
                                                        rdfs:comment "Skills are specific abilities which characters can to do in the world of game. They are affected by one or more attributes."^^xsd:string ;
                                                        rdfs:label "Skill" .


###  http://webprotege.stanford.edu/RfYd2iv36ISbO4FukwOc5P
<http://webprotege.stanford.edu/RfYd2iv36ISbO4FukwOc5P> rdf:type owl:Class ;
                                                        rdfs:subClassOf owl:Thing ;
                                                        rdfs:comment "Books about RPGs: normally contain rules, scenarios or adventures"^^xsd:string ;
                                                        rdfs:label "Book" .


###  http://webprotege.stanford.edu/RgLkIDRrYwPOlzuAbgZ20P
<http://webprotege.stanford.edu/RgLkIDRrYwPOlzuAbgZ20P> rdf:type owl:Class ;
                                                        rdfs:subClassOf owl:Thing ;
                                                        rdfs:comment "Actions are intentional events, i.e., Events with the specific purpose of satisfying (the propositional content of) some Intention of an Agent (In this sense, an Action can be said to be caused by the Intention)."^^xsd:string ;
                                                        rdfs:label "Action" ;
                                                        rdfs:seeAlso <https://ontology.com.br/ufo/ufo-c/spec/index.html> .


###  http://webprotege.stanford.edu/RgNQwN40Dphm5c3bwfi9aC
<http://webprotege.stanford.edu/RgNQwN40Dphm5c3bwfi9aC> rdf:type owl:Class ;
                                                        rdfs:comment "Foruns have many topics, each topic has a set of posts"^^xsd:string ;
                                                        rdfs:label "Topic" .


###  http://webprotege.stanford.edu/RikwLgGJ2LGt5Oth0nSQga
<http://webprotege.stanford.edu/RikwLgGJ2LGt5Oth0nSQga> rdf:type owl:Class ;
                                                        rdfs:subClassOf owl:Thing ;
                                                        rdfs:comment "Every entity is somewhere. Places are connected to each other and an entity with the correct state can transit between them."^^xsd:string ;
                                                        rdfs:label "Location" .


###  http://webprotege.stanford.edu/RoLHZFTBVkWwEBjkOnJQn5
<http://webprotege.stanford.edu/RoLHZFTBVkWwEBjkOnJQn5> rdf:type owl:Class ;
                                                        rdfs:subClassOf owl:Thing ;
                                                        rdfs:comment "A previous state which defines constraints for condition"^^xsd:string ;
                                                        rdfs:label "PreCondition"^^xsd:string .


###  http://webprotege.stanford.edu/RooQYPqs6qdydL7IIOHcg5
<http://webprotege.stanford.edu/RooQYPqs6qdydL7IIOHcg5> rdf:type owl:Class ;
                                                        rdfs:subClassOf owl:Thing ;
                                                        rdfs:comment "Missions are a set of goals for a character or group of characters. It defines events in story or gameplay."^^xsd:string ;
                                                        rdfs:label "Mission" .


###  http://www.oisrpg.com/rpg/ontology/AttributeType
:AttributeType rdf:type owl:Class ;
               owl:equivalentClass [ owl:intersectionOf ( [ rdf:type owl:Restriction ;
                                                            owl:onProperty :AttributeDomain ;
                                                            owl:cardinality "1"^^xsd:nonNegativeInteger
                                                          ]
                                                        ) ;
                                     rdf:type owl:Class
                                   ] ;
               rdfs:subClassOf owl:Thing ;
               rdfs:comment "This class is abstract type, it has not instantiate, but its children have instatiates. This is about a quality defines attributes."^^xsd:string ;
               rdfs:label "AttributeType"^^xsd:string .


###  http://www.oisrpg.com/rpg/ontology/DifferentIndividualsAtom
:DifferentIndividualsAtom rdf:type owl:Class .


###  http://www.oisrpg.com/rpg/ontology/Imp
:Imp rdf:type owl:Class .


###  http://www.oisrpg.com/rpg/ontology/IndividualPropertyAtom
:IndividualPropertyAtom rdf:type owl:Class .


###  http://www.oisrpg.com/rpg/ontology/Mental
:Mental rdf:type owl:Class ;
        rdfs:comment "Characteristics such as intelligence, perception, charisma, sanity, wisdom, will power etc among others depending rules"^^xsd:string .


###  http://www.oisrpg.com/rpg/ontology/Other
:Other rdf:type owl:Class ;
       rdfs:subClassOf owl:Thing ;
       rdfs:comment "Other variables in different contexts, like experience, life points etc"^^xsd:string .


###  http://www.oisrpg.com/rpg/ontology/Physical
:Physical rdf:type owl:Class ;
          rdfs:comment "Features such as strenght, dexterity, endurance, constitution, agility and among others depending on the rules"^^xsd:string .


#################################################################
#    Individuals
#################################################################

###  http://webprotege.stanford.edu/R1TUvFsxLDrK6cHr9Eise7
<http://webprotege.stanford.edu/R1TUvFsxLDrK6cHr9Eise7> rdf:type owl:NamedIndividual ;
                                                        rdfs:label "Faca" .


###  http://webprotege.stanford.edu/R2fgoTZKb00VpIMS4r1hal
<http://webprotege.stanford.edu/R2fgoTZKb00VpIMS4r1hal> rdf:type owl:NamedIndividual ;
                                                        rdfs:label "Campo de Aprendizes" .


###  http://webprotege.stanford.edu/R3Vc2uLhs7AG8vxTonpaO9
<http://webprotege.stanford.edu/R3Vc2uLhs7AG8vxTonpaO9> rdf:type owl:NamedIndividual ;
                                                        rdfs:label "Floresta de Payon" .


###  http://webprotege.stanford.edu/R4P9B70FKmYJFACAP2BM7W
<http://webprotege.stanford.edu/R4P9B70FKmYJFACAP2BM7W> rdf:type owl:NamedIndividual .


###  http://webprotege.stanford.edu/R4YQF2roytxDgarMmkMRJj
<http://webprotege.stanford.edu/R4YQF2roytxDgarMmkMRJj> rdf:type owl:NamedIndividual ;
                                                        rdfs:label "Carta Salgueiro" .


###  http://webprotege.stanford.edu/R7IRZcm0GibEXQ4uSnpUbKn
<http://webprotege.stanford.edu/R7IRZcm0GibEXQ4uSnpUbKn> rdf:type owl:NamedIndividual ;
                                                         rdfs:label "Raíz de Árvore" .


###  http://webprotege.stanford.edu/R7R69FSRGOp130hxgvgTgLO
<http://webprotege.stanford.edu/R7R69FSRGOp130hxgvgTgLO> rdf:type owl:NamedIndividual ;
                                                         rdfs:label "Poring" .


###  http://webprotege.stanford.edu/R7V3DDB9sWZDZRIHoVKdcyy
<http://webprotege.stanford.edu/R7V3DDB9sWZDZRIHoVKdcyy> rdf:type owl:NamedIndividual ;
                                                         rdfs:label "Asa de Mosca" .


###  http://webprotege.stanford.edu/R7ZDRUAx9M45ydVrypKBHYz
<http://webprotege.stanford.edu/R7ZDRUAx9M45ydVrypKBHYz> rdf:type owl:NamedIndividual ;
                                                         rdfs:label "Arredores de Geffen" .


###  http://webprotege.stanford.edu/R7at8XvgAsVBolVbAoq1vER
<http://webprotege.stanford.edu/R7at8XvgAsVBolVbAoq1vER> rdf:type owl:NamedIndividual ;
                                                         rdfs:label "ConsumirItem" .


###  http://webprotege.stanford.edu/R7b1GpXiARYdbHxjMwZZgb
<http://webprotege.stanford.edu/R7b1GpXiARYdbHxjMwZZgb> rdf:type owl:NamedIndividual ;
                                                        rdfs:label "Npc´s" .


###  http://webprotege.stanford.edu/R7f1XOxFJ8kDIvcgJxPTpIJ
<http://webprotege.stanford.edu/R7f1XOxFJ8kDIvcgJxPTpIJ> rdf:type owl:NamedIndividual ;
                                                         rdfs:label "Teste" .


###  http://webprotege.stanford.edu/R7tQySvwf1rp1oi18ZMIno3
<http://webprotege.stanford.edu/R7tQySvwf1rp1oi18ZMIno3> rdf:type owl:NamedIndividual ;
                                                         rdfs:label "Campo de Treinamento" .


###  http://webprotege.stanford.edu/R7xB569F1aZTdWZxWySJmtX
<http://webprotege.stanford.edu/R7xB569F1aZTdWZxWySJmtX> rdf:type owl:NamedIndividual ;
                                                         rdfs:label "Rune-Midgard" .


###  http://webprotege.stanford.edu/R80a0D1xNXkCP353KEplX3H
<http://webprotege.stanford.edu/R80a0D1xNXkCP353KEplX3H> rdf:type owl:NamedIndividual ;
                                                         rdfs:label "Chapéu de Ovo do Aprendiz" .


###  http://webprotege.stanford.edu/R80syiSZplDXBbSiSQhmijY
<http://webprotege.stanford.edu/R80syiSZplDXBbSiSQhmijY> rdf:type owl:NamedIndividual ;
                                                         rdfs:label "Muco Pegajoso" .


###  http://webprotege.stanford.edu/R87gFDHwlqX1CUplOsD0cJ3
<http://webprotege.stanford.edu/R87gFDHwlqX1CUplOsD0cJ3> rdf:type owl:NamedIndividual ;
                                                         rdfs:label "Traje do Aprendiz" .


###  http://webprotege.stanford.edu/R8NecIGjH3HMJ2cgl2uoZtL
<http://webprotege.stanford.edu/R8NecIGjH3HMJ2cgl2uoZtL> rdf:type owl:NamedIndividual ;
                                                         rdfs:label "Al de Baran" .


###  http://webprotege.stanford.edu/R8OtwJNCTanpKl5Z0X6zzmO
<http://webprotege.stanford.edu/R8OtwJNCTanpKl5Z0X6zzmO> rdf:type owl:NamedIndividual ;
                                                         rdfs:label "Funcionário Zonda" .


###  http://webprotege.stanford.edu/R8PjT5w1lXTiZzyG57kyzQ
<http://webprotege.stanford.edu/R8PjT5w1lXTiZzyG57kyzQ> rdf:type owl:NamedIndividual ;
                                                        rdfs:label "Izlude" .


###  http://webprotege.stanford.edu/R8WtZyE60BrClPIKLCnVpiM
<http://webprotege.stanford.edu/R8WtZyE60BrClPIKLCnVpiM> rdf:type owl:NamedIndividual ;
                                                         rdfs:label "Prontera" .


###  http://webprotege.stanford.edu/R8ZQSg6BD3ue55yOrycR61O
<http://webprotege.stanford.edu/R8ZQSg6BD3ue55yOrycR61O> rdf:type owl:NamedIndividual ;
                                                         rdfs:label "Pick" .


###  http://webprotege.stanford.edu/R8nQVZMInLBLl4RH46FnI8G
<http://webprotege.stanford.edu/R8nQVZMInLBLl4RH46FnI8G> rdf:type owl:NamedIndividual ;
                                                         rdfs:label "Obtendo Primeira Classe" .


###  http://webprotege.stanford.edu/R8nqcdgkqBkhOfpD0pF7FVu
<http://webprotege.stanford.edu/R8nqcdgkqBkhOfpD0pF7FVu> rdf:type owl:NamedIndividual ;
                                                         rdfs:label "ComItem" .


###  http://webprotege.stanford.edu/R8pOm6AsAmnFL91Q1aYQ6wL
<http://webprotege.stanford.edu/R8pOm6AsAmnFL91Q1aYQ6wL> rdf:type owl:NamedIndividual ;
                                                         rdfs:label "Carta Lunático" .


###  http://webprotege.stanford.edu/R8qlYBQNDW5ZyHfQ0P83Lg
<http://webprotege.stanford.edu/R8qlYBQNDW5ZyHfQ0P83Lg> rdf:type owl:NamedIndividual ;
                                                        rdfs:label "Jellopy" .


###  http://webprotege.stanford.edu/R94VQPyrmxdT1mJhYbjXGw4
<http://webprotege.stanford.edu/R94VQPyrmxdT1mJhYbjXGw4> rdf:type owl:NamedIndividual ;
                                                         rdfs:label "PegarObjeto" .


###  http://webprotege.stanford.edu/R95UVX8haAODyGIs7SYLsyk
<http://webprotege.stanford.edu/R95UVX8haAODyGIs7SYLsyk> rdf:type owl:NamedIndividual ;
                                                         rdfs:label "Carta Poring" .


###  http://webprotege.stanford.edu/R9K490nFX2NZCsK3jQPtzO0
<http://webprotege.stanford.edu/R9K490nFX2NZCsK3jQPtzO0> rdf:type owl:NamedIndividual ;
                                                         rdfs:label "Caminhar" .


###  http://webprotege.stanford.edu/R9TWdrXQMXps11bZ5wINKVm
<http://webprotege.stanford.edu/R9TWdrXQMXps11bZ5wINKVm> rdf:type owl:NamedIndividual ;
                                                         rdfs:label "Jogador" .


###  http://webprotege.stanford.edu/R9aXbE3qXoOyRmjVVLPHRIr
<http://webprotege.stanford.edu/R9aXbE3qXoOyRmjVVLPHRIr> rdf:type owl:NamedIndividual ;
                                                         rdfs:label "Capuz do Aprendiz" .


###  http://webprotege.stanford.edu/R9zchZYGDAKVJmj3otDiG7y
<http://webprotege.stanford.edu/R9zchZYGDAKVJmj3otDiG7y> rdf:type owl:NamedIndividual ;
                                                         rdfs:label "Morroc" .


###  http://webprotege.stanford.edu/RB1g3gqpIV1BRBghE0qZbDo
<http://webprotege.stanford.edu/RB1g3gqpIV1BRBghE0qZbDo> rdf:type owl:NamedIndividual ;
                                                         rdfs:label "ChonChon" .


###  http://webprotege.stanford.edu/RBADtJcJfBqZW1DkkzKZv2O
<http://webprotege.stanford.edu/RBADtJcJfBqZW1DkkzKZv2O> rdf:type owl:NamedIndividual ;
                                                         rdfs:label "Desequipar" .


###  http://webprotege.stanford.edu/RBCVw7Py5QVsId5cQpLPkWx
<http://webprotege.stanford.edu/RBCVw7Py5QVsId5cQpLPkWx> rdf:type owl:NamedIndividual ;
                                                         rdfs:label "Poção de Aprendiz" .


###  http://webprotege.stanford.edu/RBRUpfUNyjOUh66fscB7bw7
<http://webprotege.stanford.edu/RBRUpfUNyjOUh66fscB7bw7> rdf:type owl:NamedIndividual ;
                                                         rdfs:label "Trevo de 3 Folhas" .


###  http://webprotege.stanford.edu/RBS7gXlw14FWZfLP3il4La7
<http://webprotege.stanford.edu/RBS7gXlw14FWZfLP3il4La7> rdf:type owl:NamedIndividual ;
                                                         rdfs:label "Labirinto da Floresta" .


###  http://webprotege.stanford.edu/RBSCcAIPAv1lGfc2DjoUO7c
<http://webprotege.stanford.edu/RBSCcAIPAv1lGfc2DjoUO7c> rdf:type owl:NamedIndividual ;
                                                         rdfs:label "Soldado" .


###  http://webprotege.stanford.edu/RBTDvbdn8q5Av8eWxdgcjPA
<http://webprotege.stanford.edu/RBTDvbdn8q5Av8eWxdgcjPA> rdf:type owl:NamedIndividual ;
                                                         rdfs:label "Tagmar2" .


###  http://webprotege.stanford.edu/RBVGrpQMIeGwMkEBBayVaY
<http://webprotege.stanford.edu/RBVGrpQMIeGwMkEBBayVaY> rdf:type owl:NamedIndividual ;
                                                        rdfs:label "Outros Jogadores" .


###  http://webprotege.stanford.edu/RBWwsYbL4OaeuP3AhHqlIAv
<http://webprotege.stanford.edu/RBWwsYbL4OaeuP3AhHqlIAv> rdf:type owl:NamedIndividual ;
                                                         rdfs:label "Salgueiro" .


###  http://webprotege.stanford.edu/RBnq04tZIcDfzWYy98XRjpY
<http://webprotege.stanford.edu/RBnq04tZIcDfzWYy98XRjpY> rdf:type owl:NamedIndividual ;
                                                         rdfs:label "Condor" .


###  http://webprotege.stanford.edu/RBySDtwBjjx5eEealkOuWoQ
<http://webprotege.stanford.edu/RBySDtwBjjx5eEealkOuWoQ> rdf:type owl:NamedIndividual ;
                                                         rdfs:label "Sandálias de Aprendiz" .


###  http://webprotege.stanford.edu/RC6QXbG0tJ7qrfEDxIkHpnq
<http://webprotege.stanford.edu/RC6QXbG0tJ7qrfEDxIkHpnq> rdf:type owl:NamedIndividual ;
                                                         rdfs:label "Cenoura" .


###  http://webprotege.stanford.edu/RCCdoLrWkWwkWXIlxcUTNJ3
<http://webprotege.stanford.edu/RCCdoLrWkWwkWXIlxcUTNJ3> rdf:type owl:NamedIndividual ;
                                                         rdfs:label "Monstros" .


###  http://webprotege.stanford.edu/RCQzctIQIGLIvGdBEDPUkdD
<http://webprotege.stanford.edu/RCQzctIQIGLIvGdBEDPUkdD> rdf:type owl:NamedIndividual ;
                                                         rdfs:label "Ragnarök Online" .


###  http://webprotege.stanford.edu/RCSlG0bSRYCk8XtiCoK5SAl
<http://webprotege.stanford.edu/RCSlG0bSRYCk8XtiCoK5SAl> rdf:type owl:NamedIndividual ;
                                                         rdfs:label "Máscara Feliz" .


###  http://webprotege.stanford.edu/RCVX6yBf31NHwzoDCMuNafO
<http://webprotege.stanford.edu/RCVX6yBf31NHwzoDCMuNafO> rdf:type owl:NamedIndividual ;
                                                         rdfs:label "Funcionária Kafra" .


###  http://webprotege.stanford.edu/RCY2rZEPWFMdE0Qr3GQ1oOg
<http://webprotege.stanford.edu/RCY2rZEPWFMdE0Qr3GQ1oOg> rdf:type owl:NamedIndividual ;
                                                         rdfs:label "Atordoado" .


###  http://webprotege.stanford.edu/RCnlwUiLGEuZTXC4xp9HvrI
<http://webprotege.stanford.edu/RCnlwUiLGEuZTXC4xp9HvrI> rdf:type owl:NamedIndividual ;
                                                         rdfs:label "Morto" .


###  http://webprotege.stanford.edu/RCvsC9NvYuqX9zNMhiD0MXD
<http://webprotege.stanford.edu/RCvsC9NvYuqX9zNMhiD0MXD> rdf:type owl:NamedIndividual ;
                                                         rdfs:label "Equipar" .


###  http://webprotege.stanford.edu/RDD0ModVQCND8NVwlHbPrEI
<http://webprotege.stanford.edu/RDD0ModVQCND8NVwlHbPrEI> rdf:type owl:NamedIndividual ;
                                                         rdfs:label "Maçã" .


###  http://webprotege.stanford.edu/RDG7gYOFpkEdKMeCv3OWuPV
<http://webprotege.stanford.edu/RDG7gYOFpkEdKMeCv3OWuPV> rdf:type owl:NamedIndividual ;
                                                         rdfs:label "Payon" .


###  http://webprotege.stanford.edu/RDP1Gh99GcnDJkym6DW2yWO
<http://webprotege.stanford.edu/RDP1Gh99GcnDJkym6DW2yWO> rdf:type owl:NamedIndividual ;
                                                         :compostoPor <http://webprotege.stanford.edu/RCQzctIQIGLIvGdBEDPUkdD> ;
                                                         rdfs:label "Asa de Borboleta" .


###  http://webprotege.stanford.edu/RDSpRX3zfs0vaEdUsCy7ajE
<http://webprotege.stanford.edu/RDSpRX3zfs0vaEdUsCy7ajE> rdf:type owl:NamedIndividual ;
                                                         rdfs:label "Garrafa Vazia" .


###  http://webprotege.stanford.edu/RDbvRs1XuDF6SBmbOjREzZs
<http://webprotege.stanford.edu/RDbvRs1XuDF6SBmbOjREzZs> rdf:type owl:NamedIndividual ;
                                                         rdfs:label "Instrutor Brade" .


###  http://webprotege.stanford.edu/RDhWC6WNNA85VERPx0dn90H
<http://webprotege.stanford.edu/RDhWC6WNNA85VERPx0dn90H> rdf:type owl:NamedIndividual ;
                                                         rdfs:label "Tronco" .


###  http://webprotege.stanford.edu/RHDZhvOtIvFuPMxEfQ5wNk
<http://webprotege.stanford.edu/RHDZhvOtIvFuPMxEfQ5wNk> rdf:type owl:NamedIndividual ;
                                                        rdfs:label "Jinha" .


###  http://webprotege.stanford.edu/RHijNlfzfPOFIoI6IOLqxl
<http://webprotege.stanford.edu/RHijNlfzfPOFIoI6IOLqxl> rdf:type owl:NamedIndividual ;
                                                        rdfs:label "Geffen" .


###  http://webprotege.stanford.edu/RPTnoexQfEITiwmYf6t9N9
<http://webprotege.stanford.edu/RPTnoexQfEITiwmYf6t9N9> rdf:type owl:NamedIndividual ;
                                                        rdfs:label "Atacar" .


###  http://webprotege.stanford.edu/RPXxgZiZrlbr4SNnaRr7xq
<http://webprotege.stanford.edu/RPXxgZiZrlbr4SNnaRr7xq> rdf:type owl:NamedIndividual ;
                                                        rdfs:label "Lunático" .


###  http://webprotege.stanford.edu/RgGQsYaz8z5WHmBl65II1w
<http://webprotege.stanford.edu/RgGQsYaz8z5WHmBl65II1w> rdf:type owl:NamedIndividual ;
                                                        rdfs:label "Sentado" .


###  http://webprotege.stanford.edu/Rjq5MdEytsBQniOrwMXjCR
<http://webprotege.stanford.edu/Rjq5MdEytsBQniOrwMXjCR> rdf:type owl:NamedIndividual ;
                                                        rdfs:label "Em pé" .


###  http://webprotege.stanford.edu/RqIoxI7QVOPZdQrLqmttpx
<http://webprotege.stanford.edu/RqIoxI7QVOPZdQrLqmttpx> rdf:type owl:NamedIndividual ;
                                                        rdfs:label "Fabre" .


###  http://webprotege.stanford.edu/RrZpiVxOajNKpyuUajxKTH
<http://webprotege.stanford.edu/RrZpiVxOajNKpyuUajxKTH> rdf:type owl:NamedIndividual ;
                                                        rdfs:label "Batata doce" .


###  http://webprotege.stanford.edu/RtPdTKuvTrXlftK10fNRji
<http://webprotege.stanford.edu/RtPdTKuvTrXlftK10fNRji> rdf:type owl:NamedIndividual ;
                                                        rdfs:label "Envenenado" .


###  http://webprotege.stanford.edu/RxocZl2TWvVPL4prqJCnax
<http://webprotege.stanford.edu/RxocZl2TWvVPL4prqJCnax> rdf:type owl:NamedIndividual ;
                                                        rdfs:label "Deserto Sograt" .


###  http://www.oisrpg.com/rpg/ontology/AcolyteChangeClass
:AcolyteChangeClass rdf:type owl:NamedIndividual ;
                    rdfs:label "Mudança de classe: Noviço" .


###  http://www.oisrpg.com/rpg/ontology/Acrobatics
:Acrobatics rdf:type owl:NamedIndividual .


###  http://www.oisrpg.com/rpg/ontology/Agilidade
:Agilidade rdf:type owl:NamedIndividual ,
                    :Physical .


###  http://www.oisrpg.com/rpg/ontology/ArcherChangeClass
:ArcherChangeClass rdf:type owl:NamedIndividual ;
                   rdfs:label "Mudança de classe: Arqueiro" .


###  http://www.oisrpg.com/rpg/ontology/Art
:Art rdf:type owl:NamedIndividual .


###  http://www.oisrpg.com/rpg/ontology/AsaDeBorboleta
:AsaDeBorboleta rdf:type owl:NamedIndividual ;
                :carryingByPlayer :Player1 ;
                rdfs:label "Asa de Borboleta" .


###  http://www.oisrpg.com/rpg/ontology/Aura
:Aura rdf:type owl:NamedIndividual .


###  http://www.oisrpg.com/rpg/ontology/Ações_Furtivas
:Ações_Furtivas rdf:type owl:NamedIndividual .


###  http://www.oisrpg.com/rpg/ontology/Barganha
:Barganha rdf:type owl:NamedIndividual .


###  http://www.oisrpg.com/rpg/ontology/BatataDoce
:BatataDoce rdf:type owl:NamedIndividual ;
            rdfs:label "Batata doce" .


###  http://www.oisrpg.com/rpg/ontology/CamisaAlgodao
:CamisaAlgodao rdf:type owl:NamedIndividual ;
               rdfs:label "Camisa de Algodão" .


###  http://www.oisrpg.com/rpg/ontology/Carisma
:Carisma rdf:type owl:NamedIndividual ,
                  :Mental .


###  http://www.oisrpg.com/rpg/ontology/Carpintaria
:Carpintaria rdf:type owl:NamedIndividual .


###  http://www.oisrpg.com/rpg/ontology/Comércio
:Comércio rdf:type owl:NamedIndividual .


###  http://www.oisrpg.com/rpg/ontology/Destravar_Fechaduras
:Destravar_Fechaduras rdf:type owl:NamedIndividual .


###  http://www.oisrpg.com/rpg/ontology/Disguises
:Disguises rdf:type owl:NamedIndividual .


###  http://www.oisrpg.com/rpg/ontology/Engenharia
:Engenharia rdf:type owl:NamedIndividual .


###  http://www.oisrpg.com/rpg/ontology/Escalar_Superfícies
:Escalar_Superfícies rdf:type owl:NamedIndividual .


###  http://www.oisrpg.com/rpg/ontology/Escapar
:Escapar rdf:type owl:NamedIndividual .


###  http://www.oisrpg.com/rpg/ontology/Escrita
:Escrita rdf:type owl:NamedIndividual .


###  http://www.oisrpg.com/rpg/ontology/Escutar
:Escutar rdf:type owl:NamedIndividual .


###  http://www.oisrpg.com/rpg/ontology/Etiqueta
:Etiqueta rdf:type owl:NamedIndividual .


###  http://www.oisrpg.com/rpg/ontology/Falsificação
:Falsificação rdf:type owl:NamedIndividual .


###  http://www.oisrpg.com/rpg/ontology/FirstAdventure
:FirstAdventure rdf:type owl:NamedIndividual ;
                rdfs:label "Contato Inicial" .


###  http://www.oisrpg.com/rpg/ontology/Força
:Força rdf:type owl:NamedIndividual ,
                :Physical .


###  http://www.oisrpg.com/rpg/ontology/Furtar_Objetos
:Furtar_Objetos rdf:type owl:NamedIndividual .


###  http://www.oisrpg.com/rpg/ontology/Herbalismo
:Herbalismo rdf:type owl:NamedIndividual .


###  http://www.oisrpg.com/rpg/ontology/Intelecto
:Intelecto rdf:type owl:NamedIndividual ,
                    :Mental .


###  http://www.oisrpg.com/rpg/ontology/Jogatina
:Jogatina rdf:type owl:NamedIndividual .


###  http://www.oisrpg.com/rpg/ontology/Leadership
:Leadership rdf:type owl:NamedIndividual .


###  http://www.oisrpg.com/rpg/ontology/LearnFirstAid
:LearnFirstAid rdf:type owl:NamedIndividual ;
               rdfs:label "Aprender Primeiros Socorros" .


###  http://www.oisrpg.com/rpg/ontology/LearnTrickDead
:LearnTrickDead rdf:type owl:NamedIndividual ;
                rdfs:label "Aprender Fingir de Morto" .


###  http://www.oisrpg.com/rpg/ontology/Level10
:Level10 rdf:type owl:NamedIndividual .


###  http://www.oisrpg.com/rpg/ontology/Lidar_com_Animais
:Lidar_com_Animais rdf:type owl:NamedIndividual .


###  http://www.oisrpg.com/rpg/ontology/Língua
:Língua rdf:type owl:NamedIndividual .


###  http://www.oisrpg.com/rpg/ontology/MageChangeClass
:MageChangeClass rdf:type owl:NamedIndividual ;
                 rdfs:label "Mudança de classe: Mago" .


###  http://www.oisrpg.com/rpg/ontology/Malabarismo
:Malabarismo rdf:type owl:NamedIndividual .


###  http://www.oisrpg.com/rpg/ontology/Manusear_Armadilhas
:Manusear_Armadilhas rdf:type owl:NamedIndividual .


###  http://www.oisrpg.com/rpg/ontology/Medicina
:Medicina rdf:type owl:NamedIndividual .


###  http://www.oisrpg.com/rpg/ontology/MerchantChangeClass
:MerchantChangeClass rdf:type owl:NamedIndividual ;
                     rdfs:label "Mudança de classe: Mercador" .


###  http://www.oisrpg.com/rpg/ontology/Misticismo
:Misticismo rdf:type owl:NamedIndividual .


###  http://www.oisrpg.com/rpg/ontology/Montar_Animais
:Montar_Animais rdf:type owl:NamedIndividual .


###  http://www.oisrpg.com/rpg/ontology/Natação
:Natação rdf:type owl:NamedIndividual .


###  http://www.oisrpg.com/rpg/ontology/Navegação
:Navegação rdf:type owl:NamedIndividual .


###  http://www.oisrpg.com/rpg/ontology/Náutica
:Náutica rdf:type owl:NamedIndividual .


###  http://www.oisrpg.com/rpg/ontology/Observar
:Observar rdf:type owl:NamedIndividual .


###  http://www.oisrpg.com/rpg/ontology/Percepção
:Percepção rdf:type owl:NamedIndividual ,
                    :Mental .


###  http://www.oisrpg.com/rpg/ontology/Persuasão
:Persuasão rdf:type owl:NamedIndividual .


###  http://www.oisrpg.com/rpg/ontology/Player1
:Player1 rdf:type owl:NamedIndividual .


###  http://www.oisrpg.com/rpg/ontology/Religião
:Religião rdf:type owl:NamedIndividual .


###  http://www.oisrpg.com/rpg/ontology/Running
:Running rdf:type owl:NamedIndividual .


###  http://www.oisrpg.com/rpg/ontology/Sedução
:Sedução rdf:type owl:NamedIndividual .


###  http://www.oisrpg.com/rpg/ontology/Seguir_Trilhas
:Seguir_Trilhas rdf:type owl:NamedIndividual .


###  http://www.oisrpg.com/rpg/ontology/Sobrevivência
:Sobrevivência rdf:type owl:NamedIndividual .


###  http://www.oisrpg.com/rpg/ontology/SwordsmanChangeClass
:SwordsmanChangeClass rdf:type owl:NamedIndividual ;
                      rdfs:label "Mudança de classe: Espadachim" .


###  http://www.oisrpg.com/rpg/ontology/T1
:T1 rdf:type owl:NamedIndividual .


###  http://www.oisrpg.com/rpg/ontology/Tagmar2_-_Livro_de_Regras_3
:Tagmar2_-_Livro_de_Regras_3 rdf:type owl:NamedIndividual .


###  http://www.oisrpg.com/rpg/ontology/Tagmar2_-_O_Templo_e_O_Casamento
:Tagmar2_-_O_Templo_e_O_Casamento rdf:type owl:NamedIndividual .


###  http://www.oisrpg.com/rpg/ontology/TalkNPC
:TalkNPC rdf:type owl:NamedIndividual .


###  http://www.oisrpg.com/rpg/ontology/ThiefChangeClass
:ThiefChangeClass rdf:type owl:NamedIndividual ;
                  rdfs:label "Mudança de classe: Gatuno" .


###  http://www.oisrpg.com/rpg/ontology/Trabalho_em_Metal
:Trabalho_em_Metal rdf:type owl:NamedIndividual .


###  http://www.oisrpg.com/rpg/ontology/Trabalhos_Manuais
:Trabalhos_Manuais rdf:type owl:NamedIndividual .


###  http://www.oisrpg.com/rpg/ontology/Venefício
:Venefício rdf:type owl:NamedIndividual .


###  http://www.oisrpg.com/rpg/ontology/d10
:d10 rdf:type owl:NamedIndividual .


###  http://www.oisrpg.com/rpg/ontology/d20
:d20 rdf:type owl:NamedIndividual .


###  http://www.oisrpg.com/rpg/ontology/#Physical
<http://www.oisrpg.com/rpg/ontology/#Physical> rdf:type owl:NamedIndividual .


[ :argument1 <urn:swrl#x> ;
  :argument2 <urn:swrl#y>
] .



[ rdf:type :IndividualPropertyAtom ;
   :argument1 <urn:swrl#z> ;
   :argument2 <urn:swrl#y> ;
   :propertyPredicate <http://www.menthor.net/ontouml#functionalPart>
 ] .

[ rdf:type :IndividualPropertyAtom ;
   :argument1 <urn:swrl#z> ;
   :argument2 <urn:swrl#x> ;
   :propertyPredicate <http://www.menthor.net/ontouml#functionalPart>
 ] .

[ rdf:type :IndividualPropertyAtom ;
   :argument1 <urn:swrl#z> ;
   :argument2 <urn:swrl#x> ;
   :propertyPredicate <http://www.menthor.net/ontouml#collectionPart>
 ] .

[ rdf:type :IndividualPropertyAtom ;
   :argument1 <urn:swrl#y> ;
   :argument2 <urn:swrl#x> ;
   :propertyPredicate <http://www.menthor.net/ontouml#functionalPart>
 ] .

[ rdf:type :DifferentIndividualsAtom ;
   :argument1 <urn:swrl#x> ;
   :argument2 <urn:swrl#z>
 ] .


[ :argument1 <urn:swrl#z> ;
   :argument2 <urn:swrl#y> ;
   :propertyPredicate <http://www.menthor.net/ontouml#collectionPart>
 ] .

[ :argument1 <urn:swrl#y> ;
   :argument2 <urn:swrl#z>
 ] .

[ :argument1 <urn:swrl#x> ;
   :argument2 <urn:swrl#z>
 ] .

[ rdf:type :DifferentIndividualsAtom ;
   :argument1 <urn:swrl#x> ;
   :argument2 <urn:swrl#y>
 ] .

[ rdf:type :DifferentIndividualsAtom ;
   :argument1 <urn:swrl#y> ;
   :argument2 <urn:swrl#z>
 ] .

[ rdf:type :IndividualPropertyAtom ;
   :argument1 <urn:swrl#y> ;
   :argument2 <urn:swrl#x> ;
   :propertyPredicate <http://www.menthor.net/ontouml#member>
 ] .

#################################################################
#    Annotations
#################################################################

:Shoes :carringByPlayer :Rankyne .


:restritoPor rdfs:comment :Estado .

[ rdf:type owl:Axiom ;
   owl:annotatedSource :restritoPor ;
   owl:annotatedProperty rdfs:comment ;
   owl:annotatedTarget :Estado ;
   rdfs:comment :Estado
 ] .


#################################################################
#    Rules
#################################################################

[ rdf:type <http://www.w3.org/2003/11/swrl#Imp> ;
  <http://www.w3.org/2003/11/swrl#body> rdf:nil ;
  <http://www.w3.org/2003/11/swrl#head> rdf:nil
] .

###  Generated by the OWL API (version 4.5.6) https://github.com/owlcs/owlapi
